examples/MemCacheInl.v
@@ -1,244 +1,960 @@
 Require Import Ex.MemCache Lts.Notations Lts.Syntax Lts.Semantics Lts.SemFacts Lts.Refinement.
-Require Import Lts.ParametricEquiv Lts.ParametricInline Lts.ParametricInlineLtac String.
+Require Import Lts.ParametricEquiv Lts.ParametricInline String Lts.ParametricInlineLtac.
 Require Import Lts.ParametricSyntax Lib.CommonTactics Lib.Reflection Lts.Tactics List.
 
 Set Implicit Arguments.
 
-Theorem traceRefines_trans_elem: forall m1 m2 m3: Modules,
-                                   (m1 <<== m2) -> (m2 <<== m3) -> (m1 <<== m3).
-Proof.
-  intros.
-  unfold MethsT in *; rewrite idElementwiseId in *.
-  eapply traceRefines_trans; eauto.
-Qed.
+Ltac simplMod :=
+  match goal with
+    | m :=
+  ?modM: MetaModule |- _ =>
+  let mEq := fresh "mEq" in
+  let HeqmEq := fresh "HeqmEq" in
+  remember m as mEq;
+    unfold m in HeqmEq;
+    clear m;
+    cbv [inlineGenGenDm
+           inlineGenSinDm inlineSinSinDm
+           getGenGenBody
+           getGenSinBody getSinSinBody
+           appendGenGenAction appendSinSinAction appendSinGenAction
+           convNameRec nameVal nameRec isRep projT1
+           
+           ChildParent.AddrBits ChildParent.Addr ChildParent.Idx ChildParent.Data
+           ChildParent.Offset ChildParent.Line
+           ChildParent.RqToP ChildParent.RqFromC ChildParent.RsToP ChildParent.RsFromC
+           ChildParent.FromP ChildParent.ToC
+           ChildParent.rqToPPop ChildParent.rqFromCEnq ChildParent.rsToPPop
+           ChildParent.rsFromCEnq ChildParent.toCPop ChildParent.fromPEnq
+           
+           L1Cache.AddrBits L1Cache.Addr L1Cache.Tag L1Cache.Idx L1Cache.TagIdx
+           L1Cache.Data L1Cache.Offset L1Cache.Line L1Cache.RqFromProc
+           L1Cache.RsToProc L1Cache.FromP L1Cache.RqFromP L1Cache.RsFromP
+           L1Cache.RqToP L1Cache.RsToP L1Cache.rqFromProcPop L1Cache.fromPPop
+           L1Cache.rsToProcEnq L1Cache.rqToPEnq L1Cache.rsToPEnq L1Cache.readLine
+           L1Cache.writeLine L1Cache.readTag L1Cache.writeTag
+           L1Cache.readCs L1Cache.writeCs
+
+           MemCache.MIdxBits
+
+           MemDir.AddrBits MemDir.Addr MemDir.Idx MemDir.Data MemDir.Offset
+           MemDir.Line
+           MemDir.RqToP MemDir.RqFromC MemDir.RsToP
+           MemDir.RsFromC MemDir.FromP MemDir.ToC
+           MemDir.rqFromCPop MemDir.rsFromCPop MemDir.toCEnq MemDir.Dir MemDir.Dirw
+           MemDir.readLine MemDir.writeLine MemDir.readDir
+           MemDir.writeDir MemDir.Child
+
+           MemTypes.MemOp MemTypes.Child MemTypes.Data MemTypes.Line MemTypes.RqToP
+           MemTypes.RsToP MemTypes.RqFromC MemTypes.RsFromC MemTypes.ToC MemTypes.FromP
+
+           Msi.Msi RegFile.Addr StringEq.string_eq StringEq.ascii_eq Bool.eqb andb
+
+           eq_rect ret arg Struct.GetAttrType
+
+        ] in HeqmEq;
+    rewrite signature_eq in HeqmEq; unfold eq_rect in HeqmEq; simpl in HeqmEq;
+    match type of HeqmEq with
+      | ?sth = ?m => pose m; clear sth HeqmEq
+    end
+  end.
+
+Ltac simplifyMod :=
+  match goal with
+    | mRef:
+        modFromMeta (nmemCache _ _ _ _ _ _)
+                    <<== modFromMeta ?m,
+        mEquiv: forall ty, MetaModEquiv ty typeUT ?m |- _ =>
+      unfold m in mRef, mEquiv;
+  clear m;
+  cbv [inlineGenGenDm
+         inlineGenSinDm inlineSinSinDm
+         getGenGenBody
+         getGenSinBody getSinSinBody
+         appendGenGenAction appendSinSinAction appendSinGenAction
+         convNameRec nameVal nameRec isRep projT1
+         
+         ChildParent.AddrBits ChildParent.Addr ChildParent.Idx ChildParent.Data
+         ChildParent.Offset ChildParent.Line
+         ChildParent.RqToP ChildParent.RqFromC ChildParent.RsToP ChildParent.RsFromC
+         ChildParent.FromP ChildParent.ToC
+         ChildParent.rqToPPop ChildParent.rqFromCEnq ChildParent.rsToPPop
+         ChildParent.rsFromCEnq ChildParent.toCPop ChildParent.fromPEnq
+         
+         L1Cache.AddrBits L1Cache.Addr L1Cache.Tag L1Cache.Idx L1Cache.TagIdx
+         L1Cache.Data L1Cache.Offset L1Cache.Line L1Cache.RqFromProc
+         L1Cache.RsToProc L1Cache.FromP L1Cache.RqFromP L1Cache.RsFromP
+         L1Cache.RqToP L1Cache.RsToP L1Cache.rqFromProcPop L1Cache.fromPPop
+         L1Cache.rsToProcEnq L1Cache.rqToPEnq L1Cache.rsToPEnq L1Cache.readLine
+         L1Cache.writeLine L1Cache.readTag L1Cache.writeTag
+         L1Cache.readCs L1Cache.writeCs
+
+         MemCache.MIdxBits
+
+         MemDir.AddrBits MemDir.Addr MemDir.Idx MemDir.Data MemDir.Offset
+         MemDir.Line
+         MemDir.RqToP MemDir.RqFromC MemDir.RsToP
+         MemDir.RsFromC MemDir.FromP MemDir.ToC
+         MemDir.rqFromCPop MemDir.rsFromCPop MemDir.toCEnq MemDir.Dir MemDir.Dirw
+         MemDir.readLine MemDir.writeLine MemDir.readDir
+         MemDir.writeDir MemDir.Child
+
+         MemTypes.MemOp MemTypes.Child MemTypes.Data MemTypes.Line MemTypes.RqToP
+         MemTypes.RsToP MemTypes.RqFromC MemTypes.RsFromC MemTypes.ToC MemTypes.FromP
+
+         Msi.Msi RegFile.Addr StringEq.string_eq StringEq.ascii_eq Bool.eqb andb
+
+         eq_rect ret arg Struct.GetAttrType
+
+      ] in mRef, mEquiv;
+  rewrite signature_eq in mRef, mEquiv; unfold eq_rect in mRef, mEquiv;
+  simpl in mRef, mEquiv
+end;
+  match goal with
+    | mRef:
+        modFromMeta (nmemCache _ _ _ _ _ _)
+                    <<== modFromMeta ?m,
+        mEquiv: forall ty, MetaModEquiv ty typeUT ?m |- _ =>
+      let newm := fresh in
+      pose m as newm;
+        fold newm in mRef;
+        fold newm in mEquiv
+  end.
+
+
+Ltac noFilt ltac dm r :=
+  match goal with
+    | mRef:
+        modFromMeta (nmemCache _ _ _ _ _ _)
+                    <<== modFromMeta ?m,
+        mEquiv: forall ty, MetaModEquiv ty typeUT ?m |- _ =>
+      ltac dm r;
+        match goal with
+          | m'Ref:
+              modFromMeta ?m <<== modFromMeta ?m',
+              m'Equiv: forall ty, MetaModEquiv ty typeUT ?m' |- _ =>
+            apply (traceRefines_trans_elem mRef) in m'Ref; clear mRef;
+            let newm := fresh in
+            pose m' as newm;
+              fold newm in m'Ref;
+              fold newm in m'Equiv;
+              simpl in newm; clear m mEquiv
+        end
+  end; simplifyMod.
+
+Ltac ggNoFilt dm r := noFilt inlineGenDmGenRule_NoFilt dm r.
+Ltac gsNoFilt dm r := noFilt inlineSinDmGenRule_NoFilt dm r.
+Ltac ssNoFilt dm r := noFilt inlineSinDmSinRule_NoFilt dm r.
+
+Ltac ggFilt dm r := noFilt inlineGenDmGenRule_Filt dm r.
+Ltac gsFilt dm r := noFilt inlineSinDmGenRule_Filt dm r.
+Ltac ssFilt dm r := noFilt inlineSinDmSinRule_Filt dm r.
+
+
+Ltac ggNoF dm r :=
+  match goal with
+    | m := {| metaRegs :=?rgs; metaRules := ?rls; metaMeths := ?mts |} |- _ =>
+           let dmTriple := find dm (@nil MetaMeth) mts in
+           let rTriple := find r (@nil MetaRule) rls in
+           match dmTriple with
+             | (?preDm, @RepMeth ?A ?strA ?goodFn ?GenK ?getConstK
+                                 ?goodFn2 ?bdm ?dmn ?ls ?noDup, ?sufDm) =>
+               match rTriple with
+                 | (?preR, @RepRule ?A ?strA ?goodFn ?GenK ?getConstK
+                                    ?goodFn2 ?bdr ?rn ?ls ?noDup, ?sufR) =>
+                   pose
+                     {| metaRegs := rgs;
+                        metaRules := preR ++
+                                          RepRule strA goodFn getConstK goodFn2
+                                          (fun ty =>
+                                             inlineGenGenDm
+                                               (bdr ty)
+                                               (nameVal dmn) bdm) rn noDup :: sufR;
+                        metaMeths := mts |}; clear m
+               end
+           end
+  end; simplMod.
+
+Ltac ggF dm r :=
+  match goal with
+    | m := {| metaRegs :=?rgs; metaRules := ?rls; metaMeths := ?mts |} |- _ =>
+           let dmTriple := find dm (@nil MetaMeth) mts in
+           let rTriple := find r (@nil MetaRule) rls in
+           match dmTriple with
+             | (?preDm, @RepMeth ?A ?strA ?goodFn ?GenK ?getConstK
+                                 ?goodFn2 ?bdm ?dmn ?ls ?noDup, ?sufDm) =>
+               match rTriple with
+                 | (?preR, @RepRule ?A ?strA ?goodFn ?GenK ?getConstK
+                                    ?goodFn2 ?bdr ?rn ?ls ?noDup, ?sufR) =>
+                   pose
+                     {| metaRegs := rgs;
+                        metaRules := preR ++
+                                          RepRule strA goodFn getConstK goodFn2
+                                          (fun ty =>
+                                             inlineGenGenDm
+                                               (bdr ty)
+                                               (nameVal dmn) bdm) rn noDup :: sufR;
+                        metaMeths := preDm ++ sufDm |}; clear m
+               end
+           end
+  end; simplMod.
+
+Ltac gsNoF dm r :=
+  match goal with
+    | m := {| metaRegs :=?rgs; metaRules := ?rls; metaMeths := ?mts |} |- _ =>
+           let dmTriple := find dm (@nil MetaMeth) mts in
+           let rTriple := find r (@nil MetaRule) rls in
+           match dmTriple with
+             | (?preDm, @OneMeth ?bdm ?dmn, ?sufDm) =>
+               match rTriple with
+                 | (?preR, @RepRule ?A ?strA ?goodFn ?GenK ?getConstK
+                                    ?goodFn2 ?bdr ?rn ?ls ?noDup, ?sufR) =>
+                   pose
+                     {| metaRegs := rgs;
+                        metaRules := preR ++
+                                          RepRule strA goodFn getConstK goodFn2
+                                          (fun ty =>
+                                             inlineGenSinDm
+                                               (bdr ty)
+                                               (nameVal dmn) bdm) rn noDup :: sufR;
+                        metaMeths := mts |}; clear m
+               end
+           end
+  end.
+
+Ltac gsF dm r :=
+  match goal with
+    | m := {| metaRegs :=?rgs; metaRules := ?rls; metaMeths := ?mts |} |- _ =>
+           let dmTriple := find dm (@nil MetaMeth) mts in
+           let rTriple := find r (@nil MetaRule) rls in
+           match dmTriple with
+             | (?preDm, @OneMeth ?bdm ?dmn, ?sufDm) =>
+               match rTriple with
+                 | (?preR, @RepRule ?A ?strA ?goodFn ?GenK ?getConstK
+                                    ?goodFn2 ?bdr ?rn ?ls ?noDup, ?sufR) =>
+                   pose
+                     {| metaRegs := rgs;
+                        metaRules := preR ++
+                                          RepRule strA goodFn getConstK goodFn2
+                                          (fun ty =>
+                                             inlineGenSinDm
+                                               (bdr ty)
+                                               (nameVal dmn) bdm) rn noDup :: sufR;
+                        metaMeths := preDm ++ sufDm |}; clear m
+               end
+           end
+  end; simplMod.
+
+Ltac ssNoF dm r :=
+  match goal with
+    | m := {| metaRegs :=?rgs; metaRules := ?rls; metaMeths := ?mts |} |- _ =>
+           let dmTriple := find dm (@nil MetaMeth) mts in
+           let rTriple := find r (@nil MetaRule) rls in
+           match dmTriple with
+             | (?preDm, @OneMeth ?bdm ?dmn, ?sufDm) =>
+               match rTriple with
+                 | (?preR, @OneRule ?bdr ?rn, ?sufR) =>
+                   pose
+                     {| metaRegs := rgs;
+                        metaRules := preR ++
+                                          OneRule
+                                          (fun ty =>
+                                             inlineSinSinDm
+                                               (bdr ty)
+                                               (nameVal dmn) bdm) rn :: sufR;
+                        metaMeths := mts |}; clear m
+               end
+           end
+  end; simplMod.
+
+Ltac ssF dm r :=
+  match goal with
+    | m := {| metaRegs :=?rgs; metaRules := ?rls; metaMeths := ?mts |} |- _ =>
+           let dmTriple := find dm (@nil MetaMeth) mts in
+           let rTriple := find r (@nil MetaRule) rls in
+           match dmTriple with
+             | (?preDm, @OneMeth ?bdm ?dmn, ?sufDm) =>
+               match rTriple with
+                 | (?preR, @OneRule ?bdr ?rn, ?sufR) =>
+                   pose
+                     {| metaRegs := rgs;
+                        metaRules := preR ++
+                                          OneRule
+                                          (fun ty =>
+                                             inlineSinSinDm
+                                               (bdr ty)
+                                               (nameVal dmn) bdm) rn :: sufR;
+                        metaMeths := preDm ++ sufDm |}; clear m
+               end
+           end
+  end; simplMod.
+
+Ltac start_def m := let mod := fresh in pose m as mod; cbv [m] in mod.
+
+Ltac finish_def :=
+  match goal with
+    | m := ?mod: MetaModule |- _ =>
+           cbv [NativeFifo.listEltK NativeFifo.listEnq NativeFifo.listEltT] in m;
+             simpl in m; clear -m;
+             cbv [Indexer.withPrefix Indexer.prefixSymbol] in m;
+             exact mod
+  end.
+
+
+Ltac start_pf2 m mpf :=
+  let mod := fresh in
+  let pf1 := fresh in
+  let pf2 := fresh in
+  pose m as mod;
+    pose proof mpf as [pf1 pf2];
+    fold mod in pf1, pf2;
+    cbv [m] in mod.
+
+Ltac finish_pf :=
+  match goal with
+    | mRef:
+        modFromMeta (nmemCache _ _ _ _ _ _)
+                    <<== modFromMeta ?m,
+        mEquiv: forall ty, MetaModEquiv ty typeUT ?m |- _ =>
+      (abstract exact (conj mRef mEquiv))
+  end.
+
+
+
+Open Scope string.
 
 Section MemCacheInl.
   Variables IdxBits TagBits LgNumDatas LgDataBytes: nat.
   Variable Id: Kind.
 
-  Variable FifoSize: nat.
+  Variable LgNumChildren: nat.
 
-  Open Scope string.
-
-  Ltac noFilt ltac dm r :=
-    match goal with
-      | mRef:
-          modFromMeta (nmemCache IdxBits TagBits LgNumDatas LgDataBytes Id FifoSize)
-                      <<== modFromMeta ?m,
-          mEquiv: forall ty, MetaModEquiv ty typeUT ?m |- _ =>
-        ltac m mEquiv dm r;
-          match goal with
-            | m'Ref:
-                modFromMeta ?m <<== modFromMeta ?m',
-                m'Equiv: forall ty, MetaModEquiv ty typeUT ?m' |- _ =>
-                apply (traceRefines_trans_elem mRef) in m'Ref; clear mRef;
-                let newm := fresh in
-                pose m' as newm;
-                  fold newm in m'Ref;
-                  fold newm in m'Equiv;
-                  simpl in newm; clear m mEquiv
-          end
-    end.
-
-  Ltac ggNoFilt dm r := noFilt inlineGenDmGenRule_NoFilt dm r.
-  Ltac gsNoFilt dm r := noFilt inlineSinDmGenRule_NoFilt dm r.
-  Ltac ssNoFilt dm r := noFilt inlineSinDmSinRule_NoFilt dm r.
-
-  
-  
-  Ltac simplifyMod :=
-    match goal with
-      | mRef:
-          modFromMeta (nmemCache IdxBits TagBits LgNumDatas LgDataBytes Id FifoSize)
-                      <<== modFromMeta ?m,
-          mEquiv: forall ty, MetaModEquiv ty typeUT ?m |- _ =>
-        unfold m in mRef, mEquiv;
-        clear m;
-        repeat
-          unfold getGenGenBody, getGenSinBody, getSinSinBody,
-                 convNameRec, nameVal, nameRec, isRep, projT1 in mRef, mEquiv;
-        repeat autounfold with MethDefs in mRef, mEquiv;
-        rewrite signature_eq in mRef, mEquiv; unfold eq_rect in mRef, mEquiv
-    end;
-    match goal with
-      | mRef:
-          modFromMeta (nmemCache IdxBits TagBits LgNumDatas LgDataBytes Id FifoSize)
-                      <<== modFromMeta ?m,
-          mEquiv: forall ty, MetaModEquiv ty typeUT ?m |- _ =>
-        let newm := fresh in
-        pose m as newm;
-          fold newm in mRef;
-          fold newm in mEquiv
-    end.
-  
-  Ltac filt ltac dm r :=
-    match goal with
-      | mRef:
-          modFromMeta (nmemCache IdxBits TagBits LgNumDatas LgDataBytes Id FifoSize)
-                      <<== modFromMeta ?m,
-          mEquiv: forall ty, MetaModEquiv ty typeUT ?m |- _ =>
-        ltac m mEquiv dm r;
-          match goal with
-            | m'Ref:
-                modFromMeta ?m <<== modFromMeta ?m',
-                m'Equiv: forall ty, MetaModEquiv ty typeUT ?m' |- _ =>
-                apply (traceRefines_trans_elem mRef) in m'Ref; clear mRef;
-                let newm := fresh in
-                pose m' as newm;
-                  fold newm in m'Ref;
-                  fold newm in m'Equiv;
-                  simpl in newm; clear m mEquiv
-          end
-    end; simplifyMod.
-
-  Ltac ggFilt dm r := filt inlineGenDmGenRule_Filt dm r.
-  Ltac gsFilt dm r := filt inlineSinDmGenRule_Filt dm r.
-  Ltac ssFilt dm r := filt inlineSinDmSinRule_Filt dm r.
-
-  Local Notation "'LargeMetaModule'" := {| metaRegs := _;
-                                           metaRules := _;
-                                           metaMeths := _ |}.
-  
-  Definition nmemCacheInl'':
-    {m: MetaModule &
-       (modFromMeta (nmemCache IdxBits TagBits LgNumDatas
-                               LgDataBytes Id FifoSize) <<== modFromMeta m) /\
-        forall ty, MetaModEquiv ty typeUT m}.
+  Definition nmemCacheInl_flat: MetaModule.
   Proof.
-    pose (nmemCache IdxBits TagBits LgNumDatas LgDataBytes Id FifoSize) as m.
+    pose (nmemCache IdxBits TagBits LgNumDatas LgDataBytes Id LgNumChildren) as m;
 
-    repeat autounfold with ModuleDefs in m;
-    cbv [makeMetaModule getMetaFromSinNat makeSinModule getMetaFromSin
-                        sinRegs sinRules sinMeths rulesToRep regsToRep methsToRep
-                        convSinToGen concatMetaMod app metaRegs
-                        metaRules metaMeths] in m.
-    repeat (unfold Indexer.withPrefix, Indexer.prefixSymbol in m; simpl in m).
-                                                                                
-    (*
-    simpl in m; unfold concatMetaMod in m; simpl in m; unfold Indexer.withPrefix in m;
+    (*    repeat autounfold with ModuleDefs in m; *)
+    
+    cbv [
+        ChildParent.childParent
+
+          Fifo.fifo Fifo.simpleFifo
+          Fifo.fifoS Fifo.simpleFifoS
+
+          FifoCorrect.fifo FifoCorrect.nfifo
+
+          L1Cache.l1Cache l1 l1cs l1tag l1line l1Cache childParent
+
+          MemCache.memDir MemCache.mline MemCache.mdir MemCache.memDirC MemCache.memCache
+          MemCache.nl1C MemCache.nfifoRqFromC MemCache.nfifoRsFromC MemCache.nfifoToC
+          MemCache.nchildParentC MemCache.nmemCache
+
+          MemDir.memDir
+
+          NativeFifo.nativeFifo NativeFifo.nativeSimpleFifo NativeFifo.nativeFifoS
+          NativeFifo.nativeSimpleFifoS NativeFifo.nativeFifoM
+          NativeFifo.nativeSimpleFifoM
+        
+          makeMetaModule
+          getMetaFromSinNat makeSinModule getMetaFromSin
+          sinRegs sinRules sinMeths rulesToRep regsToRep methsToRep
+          convSinToGen concatMetaMod app metaRegs
+          metaRules metaMeths
+
+          Indexer.withPrefix Indexer.prefixSymbol
+
+          ChildParent.AddrBits ChildParent.Addr ChildParent.Idx ChildParent.Data
+          ChildParent.Offset ChildParent.Line
+          ChildParent.RqToP ChildParent.RqFromC ChildParent.RsToP ChildParent.RsFromC
+          ChildParent.FromP ChildParent.ToC
+          ChildParent.rqToPPop ChildParent.rqFromCEnq ChildParent.rsToPPop
+          ChildParent.rsFromCEnq ChildParent.toCPop ChildParent.fromPEnq
+          
+          L1Cache.AddrBits L1Cache.Addr L1Cache.Tag L1Cache.Idx L1Cache.TagIdx
+          L1Cache.Data L1Cache.Offset L1Cache.Line L1Cache.RqFromProc
+          L1Cache.RsToProc L1Cache.FromP L1Cache.RqFromP L1Cache.RsFromP
+          L1Cache.RqToP L1Cache.RsToP L1Cache.rqFromProcPop L1Cache.fromPPop
+          L1Cache.rsToProcEnq L1Cache.rqToPEnq L1Cache.rsToPEnq L1Cache.readLine
+          L1Cache.writeLine L1Cache.readTag L1Cache.writeTag L1Cache.readCs L1Cache.writeCs
+
+          L1Cache.RqFromProc L1Cache.rqFromProcFirst
+
+          MemCache.MIdxBits
+
+          MemDir.AddrBits MemDir.Addr MemDir.Idx MemDir.Data MemDir.Offset MemDir.Line
+          MemDir.RqToP MemDir.RqFromC MemDir.RsToP MemDir.RsFromC MemDir.FromP MemDir.ToC
+          MemDir.rqFromCPop MemDir.rsFromCPop MemDir.toCEnq MemDir.Dir MemDir.Dirw
+          MemDir.readLine MemDir.writeLine MemDir.readDir MemDir.writeDir MemDir.Child
+
+          MemTypes.MemOp MemTypes.Child MemTypes.Data MemTypes.Line
+          MemTypes.RsToP MemTypes.RqFromC MemTypes.RsFromC MemTypes.ToC
+
+          RegFile.regFileM RegFile.regFileS RegFile.regFile
+
+          nfifoRqToP nfifoRsToP nfifoFromP
+
+          String.append
+
+          fullType
+
+          ret arg
+
+          projT1 projT2
+
+          (*
+          Struct.attrName Struct.attrType
+
+          
+          getDefaultConst
+          makeConst
+
+          RegFile.DataArray Msi.Msi
+
+          getDefaultConstBit
+
+          MemTypes.RqToP MemTypes.RsToProc MemTypes.FromP
+          Void
+
+          NativeFifo.nativeEnqS
+          MemTypes.RqFromProc
+
+          NativeFifo.listEltK
+          NativeFifo.nativeDeqS
+          NativeFifo.nativeFirstEltS
+           *)
+      ] in m;
     simpl in m.
-     *)
-    assert (mRef: modFromMeta (nmemCache IdxBits TagBits LgNumDatas LgDataBytes Id FifoSize)
-                                <<== modFromMeta m) by
-        (unfold MethsT; rewrite @idElementwiseId; apply traceRefines_refl).
-    assert (mEquiv: forall ty, MetaModEquiv ty typeUT m) by kequiv.
 
-    ssNoFilt "read.mline" "hit".
-    simplifyMod; ssFilt "read.mline" "deferred".
+    finish_def.
+  Defined.
 
-    ssNoFilt "read.mcs" "hit".
+  Theorem nmemCacheInl_flat_pf:
+    (modFromMeta (nmemCache IdxBits TagBits LgNumDatas
+                            LgDataBytes Id LgNumChildren) <<== modFromMeta nmemCacheInl_flat) /\
+    forall ty, MetaModEquiv ty typeUT nmemCacheInl_flat.
+  Proof.
+    assert (mRef: modFromMeta
+                    (nmemCache IdxBits TagBits LgNumDatas LgDataBytes Id LgNumChildren)
+                    <<== modFromMeta nmemCacheInl_flat) by
+        (abstract (cbv [nmemCacheInl_flat]; unfold MethsT;
+                   rewrite @idElementwiseId; apply traceRefines_refl)).
+    assert (mEquiv: forall ty, MetaModEquiv ty typeUT nmemCacheInl_flat)
+      by (abstract (cbv [nmemCacheInl_flat];
+                    kequiv)).
+
+    finish_pf.
+  Qed.
+
+  Definition nmemCacheInl_1: MetaModule.
+  Proof.
+    start_def nmemCacheInl_flat.
+
+    ssF "read.mline" "deferred".
+  
+    ssNoF "read.mcs" "missByState".
+    ssNoF "read.mcs" "dwnRq".
+    ssNoF "read.mcs" "dwnRs".
+    ssF "read.mcs" "deferred".
+
+    ssF "write.mline" "dwnRs".
+
+    ssNoF "write.mcs" "dwnRs".
+    ssF "write.mcs" "deferred".
+
+    finish_def.
+  Defined.
+
+  Theorem nmemCacheInl_1_pf:
+    (modFromMeta (nmemCache IdxBits TagBits LgNumDatas
+                            LgDataBytes Id LgNumChildren) <<== modFromMeta nmemCacheInl_1) /\
+    forall ty, MetaModEquiv ty typeUT nmemCacheInl_1.
+  Proof.
+    start_pf2 nmemCacheInl_flat nmemCacheInl_flat_pf.
+    
+    ssFilt "read.mline" "deferred".
+  
     ssNoFilt "read.mcs" "missByState".
     ssNoFilt "read.mcs" "dwnRq".
     ssNoFilt "read.mcs" "dwnRs".
-    simplifyMod; ssFilt "read.mcs" "deferred".
+    ssFilt "read.mcs" "deferred".
 
     ssFilt "write.mline" "dwnRs".
 
-    ssNoFilt "write.mcs" "hit".
     ssNoFilt "write.mcs" "dwnRs".
-    simplifyMod; ssFilt "write.mcs" "deferred".
+    ssFilt "write.mcs" "deferred".
 
-    ssNoFilt "enq.toChild" "hit".
-    ssNoFilt "enq.toChild" "dwnRq".
-    simplifyMod; ssFilt "enq.toChild" "deferred".
+    finish_pf.
+  Qed.
+
+  Definition nmemCacheInl_2: MetaModule.
+  Proof.
+
+    start_def nmemCacheInl_1.
+    ssNoF "enq.toChild" "dwnRq".
+    ssF "enq.toChild" "deferred".
+
+    ssNoF "firstElt.rqFromChild" "missByState".
+    ssF "firstElt.rqFromChild" "dwnRq".
     
-    ssNoFilt "deq.rqFromChild" "hit".
-    ssNoFilt "deq.rqFromChild" "missByState".
-    simplifyMod; ssFilt "deq.rqFromChild" "deferred".
+    ssF "deq.rqFromChild" "deferred".
+
+    ssF "deq.rsFromChild" "dwnRs".
+
+    finish_def.
+  Defined.
+
+  Theorem nmemCacheInl_2_pf:
+    (modFromMeta (nmemCache IdxBits TagBits LgNumDatas
+                            LgDataBytes Id LgNumChildren) <<== modFromMeta nmemCacheInl_2) /\
+    forall ty, MetaModEquiv ty typeUT nmemCacheInl_2.
+  Proof.
+
+    start_pf2 nmemCacheInl_1 nmemCacheInl_1_pf.
+    
+    ssNoFilt "enq.toChild" "dwnRq".
+    ssFilt "enq.toChild" "deferred".
+
+    ssNoFilt "firstElt.rqFromChild" "missByState".
+    ssFilt "firstElt.rqFromChild" "dwnRq".
+    
+    ssFilt "deq.rqFromChild" "deferred".
 
     ssFilt "deq.rsFromChild" "dwnRs".
+
+    finish_pf.
+  Qed.
+
+  Definition nmemCacheInl_3: MetaModule.
+  Proof.
+
+    start_def nmemCacheInl_2.
+    gsF "enq.rsFromChild" "rsFromCToP".
+
+    gsF "enq.rqFromChild" "rqFromCToP".
     
+    gsF "deq.toChild" "fromPToC".
+
+    finish_def.
+  Defined.
+
+  Theorem nmemCacheInl_3_pf:
+    (modFromMeta (nmemCache IdxBits TagBits LgNumDatas
+                            LgDataBytes Id LgNumChildren) <<== modFromMeta nmemCacheInl_3) /\
+    forall ty, MetaModEquiv ty typeUT nmemCacheInl_3.
+  Proof.
+
+    start_pf2 nmemCacheInl_2 nmemCacheInl_2_pf.
     gsFilt "enq.rsFromChild" "rsFromCToP".
 
     gsFilt "enq.rqFromChild" "rqFromCToP".
     
     gsFilt "deq.toChild" "fromPToC".
+
+    finish_pf.
+  Defined.
+  
+
+  
+  Definition nmemCacheInl_4: MetaModule.
+  Proof.
+    start_def nmemCacheInl_3.
+
+    ggNoF "read.cs" "l1MissByState".
+    ggNoF "read.cs" "l1MissByLine".
+    ggNoF "read.cs" "l1Hit".    
+    ggNoF "read.cs" "writeback".
+    ggNoF "read.cs" "upgRq".
+    ggNoF "read.cs" "upgRs".
+
+    finish_def.
+  Defined.
+
+  Definition nmemCacheInl_4_5: MetaModule.
+  Proof.
+    start_def nmemCacheInl_4.
     
-    ggNoFilt "read.cs" "ldHit".
-    ggNoFilt "read.cs" "stHit".
+    ggNoF "read.cs" "ld".
+    ggNoF "read.cs" "st".
+    ggNoF "read.cs" "drop".
+    ggF "read.cs" "pProcess".
+
+    finish_def.
+  Defined.
+
+  Theorem nmemCacheInl_4_pf:
+    (modFromMeta (nmemCache IdxBits TagBits LgNumDatas
+                            LgDataBytes Id LgNumChildren) <<== modFromMeta nmemCacheInl_4) /\
+    forall ty, MetaModEquiv ty typeUT nmemCacheInl_4.
+  Proof.
+
+    start_pf2 nmemCacheInl_3 nmemCacheInl_3_pf.
+
     ggNoFilt "read.cs" "l1MissByState".
     ggNoFilt "read.cs" "l1MissByLine".
+    ggNoFilt "read.cs" "l1Hit".    
     ggNoFilt "read.cs" "writeback".
     ggNoFilt "read.cs" "upgRq".
     ggNoFilt "read.cs" "upgRs".
-    ggNoFilt "read.cs" "ldDeferred".
-    ggNoFilt "read.cs" "stDeferred".
-    ggNoFilt "read.cs" "drop".
-    simplifyMod; ggFilt "read.cs" "pProcess".
 
-    ggNoFilt "read.tag" "ldHit".
-    ggNoFilt "read.tag" "stHit".
+    finish_pf.
+  Qed.
+    
+  Theorem nmemCacheInl_4_5_pf:
+    (modFromMeta (nmemCache IdxBits TagBits LgNumDatas
+                            LgDataBytes Id LgNumChildren) <<== modFromMeta nmemCacheInl_4_5) /\
+    forall ty, MetaModEquiv ty typeUT nmemCacheInl_4_5.
+  Proof.
+    start_pf2 nmemCacheInl_4 nmemCacheInl_4_pf.
+
+    ggNoFilt "read.cs" "ld".
+    ggNoFilt "read.cs" "st".
+    ggNoFilt "read.cs" "drop".
+    ggFilt "read.cs" "pProcess".
+
+    finish_pf.
+  Qed. 
+End MemCacheInl.
+
+Section MemCacheInl2.
+
+  Variables IdxBits TagBits LgNumDatas LgDataBytes: nat.
+  Variable Id: Kind.
+
+  Variable LgNumChildren: nat.
+
+  Definition nmemCacheInl_4_5': MetaModule.
+  Proof.
+    pose (nmemCacheInl_4_5 IdxBits TagBits LgNumDatas LgDataBytes Id LgNumChildren) as sth.
+    unfold nmemCacheInl_4_5 in sth.
+    match goal with
+      | m := ?mod |- _ => exact mod
+    end.
+  Defined.
+
+  Theorem nmemCacheInl_4_5'_pf:
+    (modFromMeta (nmemCache IdxBits TagBits LgNumDatas
+                            LgDataBytes Id LgNumChildren) <<== modFromMeta nmemCacheInl_4_5') /\
+    forall ty, MetaModEquiv ty typeUT nmemCacheInl_4_5'.
+  Proof.
+    eapply nmemCacheInl_4_5_pf; eauto.
+  Qed.
+  
+
+  
+  Definition nmemCacheInl_5: MetaModule.
+  Proof.
+    start_def nmemCacheInl_4_5'.
+    
+    ggNoF "read.tag" "l1MissByState".
+    ggNoF "read.tag" "l1MissByLine".
+    ggNoF "read.tag" "l1Hit".    
+    ggNoF "read.tag" "writeback".
+    ggNoF "read.tag" "drop".
+    ggF "read.tag" "pProcess".
+
+    finish_def.
+  Defined.
+
+  Theorem nmemCacheInl_5_pf:
+    (modFromMeta (nmemCache IdxBits TagBits LgNumDatas
+                            LgDataBytes Id LgNumChildren) <<== modFromMeta nmemCacheInl_5) /\
+    forall ty, MetaModEquiv ty typeUT nmemCacheInl_5.
+  Proof.
+    start_pf2 nmemCacheInl_4_5' nmemCacheInl_4_5'_pf.
+    
     ggNoFilt "read.tag" "l1MissByState".
     ggNoFilt "read.tag" "l1MissByLine".
+    ggNoFilt "read.tag" "l1Hit".    
     ggNoFilt "read.tag" "writeback".
     ggNoFilt "read.tag" "drop".
-    simplifyMod; ggFilt "read.tag" "pProcess".
+    ggFilt "read.tag" "pProcess".
 
-    ggNoFilt "read.line" "ldHit".
-    ggNoFilt "read.line" "stHit".
+    finish_pf.
+  Qed.
+End MemCacheInl2.
+  
+Section MemCacheInl3.
+
+  Variables IdxBits TagBits LgNumDatas LgDataBytes: nat.
+  Variable Id: Kind.
+
+  Variable LgNumChildren: nat.
+
+  Definition nmemCacheInl_5': MetaModule.
+  Proof.
+    pose (nmemCacheInl_5 IdxBits TagBits LgNumDatas LgDataBytes Id LgNumChildren) as sth.
+    unfold nmemCacheInl_5 in sth.
+    match goal with
+      | m := ?mod |- _ => exact mod
+    end.
+  Defined.
+
+  Theorem nmemCacheInl_5'_pf:
+    (modFromMeta (nmemCache IdxBits TagBits LgNumDatas
+                            LgDataBytes Id LgNumChildren) <<== modFromMeta nmemCacheInl_5') /\
+    forall ty, MetaModEquiv ty typeUT nmemCacheInl_5'.
+  Proof.
+    eapply nmemCacheInl_5_pf; eauto.
+  Qed.
+  
+
+  Definition nmemCacheInl_6: MetaModule.
+  Proof.
+    start_def nmemCacheInl_5'.
+    ggNoF "read.line" "writeback".
+    ggNoF "read.line" "ld".
+    ggNoF "read.line" "st".
+    ggF "read.line" "pProcess".
+    finish_def.
+  Defined.
+
+  Definition nmemCacheInl_6_3: MetaModule.
+  Proof.
+    start_def nmemCacheInl_6.
+    ggNoF "write.cs" "writeback".
+    ggNoF "write.cs" "upgRs".
+    finish_def.
+  Defined.
+
+  Definition nmemCacheInl_6_6: MetaModule.
+  Proof.
+    start_def nmemCacheInl_6_3.
+    ggF "write.cs" "pProcess".
+
+    finish_def.
+  Defined.
+
+  Theorem nmemCacheInl_6_pf:
+    (modFromMeta (nmemCache IdxBits TagBits LgNumDatas
+                            LgDataBytes Id LgNumChildren) <<== modFromMeta nmemCacheInl_6) /\
+    forall ty, MetaModEquiv ty typeUT nmemCacheInl_6.
+  Proof.
+    start_pf2 nmemCacheInl_5' nmemCacheInl_5'_pf.
+    
     ggNoFilt "read.line" "writeback".
-    ggNoFilt "read.line" "ldDeferred".
-    ggNoFilt "read.line" "stDeferred".
-    ggNoFilt "read.line" "stDeferred".
-    simplifyMod; ggFilt "read.line" "pProcess".
+    ggNoFilt "read.line" "ld".
+    ggNoFilt "read.line" "st".
+    ggFilt "read.line" "pProcess".
+    finish_pf.
+  Qed.
 
+  Theorem nmemCacheInl_6_3_pf:
+    (modFromMeta (nmemCache IdxBits TagBits LgNumDatas
+                            LgDataBytes Id LgNumChildren) <<== modFromMeta nmemCacheInl_6_3) /\
+    forall ty, MetaModEquiv ty typeUT nmemCacheInl_6_3.
+  Proof.
+    start_pf2 nmemCacheInl_6 nmemCacheInl_6_pf.
+    
     ggNoFilt "write.cs" "writeback".
     ggNoFilt "write.cs" "upgRs".
 
-    simplifyMod; ggFilt "write.cs" "pProcess".
+    finish_pf.
+  Qed.
 
-    ggFilt "write.tag" "upgRs".
-
-    ggNoFilt "write.line" "stHit".
-    ggNoFilt "write.line" "upgRs".
-    simplifyMod; ggFilt "write.line" "stDeferred".
-
-    ggNoFilt "deq.fromParent" "upgRs".
-    ggNoFilt "deq.fromParent" "drop".
-    simplifyMod; ggFilt "deq.fromParent" "pProcess".
+  Theorem nmemCacheInl_6_6_pf:
+    (modFromMeta (nmemCache IdxBits TagBits LgNumDatas
+                            LgDataBytes Id LgNumChildren) <<== modFromMeta nmemCacheInl_6_6) /\
+    forall ty, MetaModEquiv ty typeUT nmemCacheInl_6_6.
+  Proof.
+    start_pf2 nmemCacheInl_6_3 nmemCacheInl_6_3_pf.
     
-    ggNoFilt "enq.rsToProc" "ldHit".
-    ggNoFilt "enq.rsToProc" "stHit".
-    ggNoFilt "enq.rsToProc" "ldDeferred".
-    simplifyMod; ggFilt "enq.rsToProc" "stDeferred".
+    ggFilt "write.cs" "pProcess".
+    finish_pf.
+  Qed.
+End MemCacheInl3.
+  
+Section MemCacheInl4.
 
-    ggFilt "enq.rqToParent" "upgRq".
+  Variables IdxBits TagBits LgNumDatas LgDataBytes: nat.
+  Variable Id: Kind.
 
-    ggNoFilt "enq.rsToParent" "writeback".
-    simplifyMod; ggFilt "enq.rsToParent" "pProcess".
+  Variable LgNumChildren: nat.
 
-    ggFilt "deq.rqToParent" "rqFromCToP".
-    ggFilt "deq.rsToParent" "rsFromCToP".
-    ggFilt "enq.fromParent" "fromPToC".
-    
+  Definition nmemCacheInl_6_6': MetaModule.
+  Proof.
+    pose (nmemCacheInl_6_6 IdxBits TagBits LgNumDatas LgDataBytes Id LgNumChildren) as sth.
+    unfold nmemCacheInl_6_6 in sth.
     match goal with
-      | mRef:
-          modFromMeta (nmemCache IdxBits TagBits LgNumDatas LgDataBytes Id FifoSize)
-                      <<== modFromMeta ?m,
-          mEquiv: forall ty, MetaModEquiv ty typeUT ?m |- _ =>
-        exact (existT _ m (conj mRef mEquiv))
+      | m := ?mod |- _ => exact mod
     end.
-
   Defined.
 
-  Definition nmemCacheInl := projT1 nmemCacheInl''.
-
-  Theorem nmemCacheInl_refines:
-    modFromMeta (nmemCache IdxBits TagBits LgNumDatas
-                           LgDataBytes Id FifoSize) <<== modFromMeta nmemCacheInl.
+  Theorem nmemCacheInl_6_6'_pf:
+    (modFromMeta (nmemCache IdxBits TagBits LgNumDatas
+                            LgDataBytes Id LgNumChildren) <<== modFromMeta nmemCacheInl_6_6') /\
+    forall ty, MetaModEquiv ty typeUT nmemCacheInl_6_6'.
   Proof.
-    pose proof (projT2 nmemCacheInl'') as sth.
-    destruct sth.
-    assumption.
+    eapply nmemCacheInl_6_6_pf; eauto.
+  Qed.
+  
+
+  Definition nmemCacheInl_7: MetaModule.
+  Proof.
+    start_def nmemCacheInl_6_6'.
+    ggF "write.tag" "upgRs".
+    finish_def.
+  Defined.
+
+  Definition nmemCacheInl_7_3: MetaModule.
+  Proof.
+    start_def nmemCacheInl_7.
+    ggNoF "write.line" "upgRs".
+    ggF "write.line" "st".
+    finish_def.
+  Defined.
+  
+  Definition nmemCacheInl_7_7: MetaModule.
+  Proof.
+    start_def nmemCacheInl_7_3.
+    ggNoF "deq.fromParent" "upgRs".
+    ggNoF "deq.fromParent" "drop".
+    ggF "deq.fromParent" "pProcess".
+    finish_def.
+  Defined.
+
+  Theorem nmemCacheInl_7_pf:
+    (modFromMeta (nmemCache IdxBits TagBits LgNumDatas
+                            LgDataBytes Id LgNumChildren) <<== modFromMeta nmemCacheInl_7) /\
+    forall ty, MetaModEquiv ty typeUT nmemCacheInl_7.
+  Proof.
+    start_pf2 nmemCacheInl_6_6' nmemCacheInl_6_6'_pf.
+    ggFilt "write.tag" "upgRs".
+    finish_pf.
   Qed.
 
-  Theorem nmemCacheInl_equiv:
+  Theorem nmemCacheInl_7_3_pf:
+    (modFromMeta (nmemCache IdxBits TagBits LgNumDatas
+                            LgDataBytes Id LgNumChildren) <<== modFromMeta nmemCacheInl_7_3) /\
+    forall ty, MetaModEquiv ty typeUT nmemCacheInl_7_3.
+  Proof.
+    start_pf2 nmemCacheInl_7 nmemCacheInl_7_pf.
+    ggNoFilt "write.line" "upgRs".
+    ggFilt "write.line" "st".
+    finish_pf.
+  Qed.
+
+  Theorem nmemCacheInl_7_7_pf:
+    (modFromMeta (nmemCache IdxBits TagBits LgNumDatas
+                            LgDataBytes Id LgNumChildren) <<== modFromMeta nmemCacheInl_7_7) /\
+    forall ty, MetaModEquiv ty typeUT nmemCacheInl_7_7.
+  Proof.
+    start_pf2 nmemCacheInl_7_3 nmemCacheInl_7_3_pf.
+    ggNoFilt "deq.fromParent" "upgRs".
+    ggNoFilt "deq.fromParent" "drop".
+    ggFilt "deq.fromParent" "pProcess".
+    finish_pf.
+  Qed.
+End MemCacheInl4.
+
+Section MemCacheInl5.
+  Variables IdxBits TagBits LgNumDatas LgDataBytes: nat.
+  Variable Id: Kind.
+
+  Variable LgNumChildren: nat.
+
+  Definition nmemCacheInl_7_7': MetaModule.
+  Proof.
+    pose (nmemCacheInl_7_7 IdxBits TagBits LgNumDatas LgDataBytes Id LgNumChildren) as sth.
+    unfold nmemCacheInl_7_7 in sth.
+    match goal with
+      | m := ?mod |- _ => exact mod
+    end.
+  Defined.
+
+  Theorem nmemCacheInl_7_7'_pf:
+    (modFromMeta (nmemCache IdxBits TagBits LgNumDatas
+                            LgDataBytes Id LgNumChildren) <<== modFromMeta nmemCacheInl_7_7') /\
+    forall ty, MetaModEquiv ty typeUT nmemCacheInl_7_7'.
+  Proof.
+    eapply nmemCacheInl_7_7_pf; eauto.
+  Qed.
+  
+
+  Definition nmemCacheInl_8: MetaModule.
+  Proof.
+    start_def nmemCacheInl_7_7'.
+    ggF "enq.rqToParent" "upgRq".
+    finish_def.
+  Defined.
+
+  Definition nmemCacheInl_9: MetaModule.
+  Proof.
+    start_def nmemCacheInl_8.
+    ggNoF "enq.rsToParent" "writeback".
+    ggF "enq.rsToParent" "pProcess".
+    finish_def.
+  Defined.
+
+  Definition nmemCacheInl_10: MetaModule.
+  Proof.
+    start_def nmemCacheInl_9.
+    ggF "deq.rqToParent" "rqFromCToP".
+    finish_def.
+  Defined.
+    
+  Definition nmemCacheInl_11: MetaModule.
+  Proof.
+    start_def nmemCacheInl_10.
+    ggF "deq.rsToParent" "rsFromCToP".
+    finish_def.
+  Defined.
+
+  
+  Definition nmemCacheInl: MetaModule.
+  Proof.
+    start_def nmemCacheInl_11.
+    ggF "enq.fromParent" "fromPToC".
+    finish_def.
+  Defined.
+
+  Theorem nmemCacheInl_8_pf:
+    (modFromMeta (nmemCache IdxBits TagBits LgNumDatas
+                            LgDataBytes Id LgNumChildren) <<== modFromMeta nmemCacheInl_8) /\
+    forall ty, MetaModEquiv ty typeUT nmemCacheInl_8.
+  Proof.
+    start_pf2 nmemCacheInl_7_7' nmemCacheInl_7_7'_pf.
+    ggFilt "enq.rqToParent" "upgRq".
+    finish_pf.
+  Qed.
+
+  Theorem nmemCacheInl_9_pf:
+    (modFromMeta (nmemCache IdxBits TagBits LgNumDatas
+                            LgDataBytes Id LgNumChildren) <<== modFromMeta nmemCacheInl_9) /\
+    forall ty, MetaModEquiv ty typeUT nmemCacheInl_9.
+  Proof.
+    start_pf2 nmemCacheInl_8 nmemCacheInl_8_pf.
+    ggNoFilt "enq.rsToParent" "writeback".
+    ggFilt "enq.rsToParent" "pProcess".
+    finish_pf.
+  Qed.
+
+  Theorem nmemCacheInl_10_pf:
+    (modFromMeta (nmemCache IdxBits TagBits LgNumDatas
+                            LgDataBytes Id LgNumChildren) <<== modFromMeta nmemCacheInl_10) /\
+    forall ty, MetaModEquiv ty typeUT nmemCacheInl_10.
+  Proof.
+    start_pf2 nmemCacheInl_9 nmemCacheInl_9_pf.
+    ggFilt "deq.rqToParent" "rqFromCToP".
+    finish_pf.
+  Qed.
+  
+  Theorem nmemCacheInl_11_pf:
+    (modFromMeta (nmemCache IdxBits TagBits LgNumDatas
+                            LgDataBytes Id LgNumChildren) <<== modFromMeta nmemCacheInl_11) /\
+    forall ty, MetaModEquiv ty typeUT nmemCacheInl_11.
+  Proof.
+    start_pf2 nmemCacheInl_10 nmemCacheInl_10_pf.
+    ggFilt "deq.rsToParent" "rsFromCToP".
+    finish_pf.
+  Qed.
+
+  Theorem nmemCacheInl_pf:
+    (modFromMeta (nmemCache IdxBits TagBits LgNumDatas
+                            LgDataBytes Id LgNumChildren) <<== modFromMeta nmemCacheInl) /\
     forall ty, MetaModEquiv ty typeUT nmemCacheInl.
   Proof.
-    pose proof (projT2 nmemCacheInl'') as sth.
-    destruct sth.
-    assumption.
+    start_pf2 nmemCacheInl_11 nmemCacheInl_11_pf.
+    ggFilt "enq.fromParent" "fromPToC".
+    finish_pf.
   Qed.
-
-  Close Scope string.
-End MemCacheInl.
+End MemCacheInl5.
