src/ParametricInlineLtac.v
@@ -1,197 +1,173 @@
 Require Import ParametricInline List ParametricSyntax String Syntax
-        Lib.CommonTactics Lib.Reflection Tactics.
+        Lib.CommonTactics Lib.Reflection Tactics ParametricEquiv.
 
-Fixpoint findDm dm pre ls :=
+Open Scope string.
+
+Ltac app_ltac ls x :=
   match ls with
-    | nil => None
-    | OneMeth bd {| nameVal := dmName; goodName := pf |} :: xs =>
-      match string_dec dmName dm with
-        | left isEq =>
-          Some (pre, OneMeth bd {| nameVal := dm; goodName := match isEq with
-                                                                | eq_refl => pf
-                                                              end |}, xs)
-        | right _ =>
-          findDm dm (pre ++ OneMeth bd {| nameVal := dmName; goodName := pf |} :: nil) xs
-      end
-    | RepMeth A strA goodFn GenK getConstK goodFn2 bd
-              {| nameVal := dmName; goodName := pf |} _ noDup :: xs =>
-      match string_dec dmName dm with
-        | left isEq =>
-          Some (pre, RepMeth strA goodFn getConstK
-                             goodFn2 bd {| nameVal := dm; goodName :=
-                                                            match isEq with
-                                                              | eq_refl => pf
-                                                            end |} noDup, xs)
-        | right _ =>
-          findDm dm (pre ++ RepMeth strA goodFn getConstK goodFn2
-                         bd {| nameVal := dmName; goodName := pf |} noDup :: nil) xs
+    | ?y :: ?ys =>
+      let ns := app_ltac ys x in
+      constr:(y :: ns)
+    | nil => constr:(x :: nil)
+  end.
+
+Ltac find dm pre ls :=
+  match ls with
+    | ?x :: ?xs =>
+      match x with
+        | context[dm] =>
+          constr:(pre, x, xs)
+        | _ =>
+          let y := app_ltac pre x in
+          find dm y xs
       end
   end.
 
-Fixpoint findR dm pre ls :=
-  match ls with
-    | nil => None
-    | OneRule bd {| nameVal := dmName; goodName := pf |} :: xs =>
-      match string_dec dmName dm with
-        | left isEq =>
-          Some (pre, OneRule bd {| nameVal := dm; goodName := match isEq with
-                                                                | eq_refl => pf
-                                                              end |}, xs)
-        | right _ =>
-          findR dm (pre ++ OneRule bd {| nameVal := dmName; goodName := pf |} :: nil) xs
-      end
-    | RepRule A strA goodFn GenK getConstK goodFn2 bd
-              {| nameVal := dmName; goodName := pf |} _ noDup :: xs =>
-      match string_dec dmName dm with
-        | left isEq =>
-          Some (pre, RepRule strA goodFn getConstK
-                             goodFn2 bd {| nameVal := dm; goodName :=
-                                                            match isEq with
-                                                              | eq_refl => pf
-                                                            end |} noDup, xs)
-        | right _ =>
-          findR dm (pre ++ RepRule strA goodFn getConstK goodFn2
-                        bd {| nameVal := dmName; goodName := pf |} noDup :: nil) xs
-      end
+Ltac inlineGenDmGenRule_NoFilt dm r :=
+  match goal with
+    | m := {| metaRegs := _; metaRules := ?rls; metaMeths := ?mts |},
+           mEquiv: forall ty, MetaModEquiv ty typeUT _ |- _ =>
+           let noDupMeth := fresh in
+           let noDupRule := fresh in
+           assert (noDupMeth: NoDup (map getMetaMethName mts)) by
+               ( (subst; simpl; clear; noDup_tac));
+             assert (noDupRule: NoDup (map getMetaRuleName rls)) by
+               ( (subst; simpl; clear; noDup_tac));
+             let dmTriple := find dm (@nil MetaMeth) mts in
+             let rTriple := find r (@nil MetaRule) rls in
+             match dmTriple with
+               | (?preDm, @RepMeth ?A ?strA ?goodFn ?GenK ?getConstK
+                                   ?goodFn2 ?bdm ?dmn ?ls ?noDup, ?sufDm) =>
+                 match rTriple with
+                   | (?preR, @RepRule ?A ?strA ?goodFn ?GenK ?getConstK
+                                      ?goodFn2 ?bdr ?rn ?ls ?noDup, ?sufR) =>
+                     pose proof (@inlineGenGenDmToRule_traceRefines_NoFilt
+                                   m A strA goodFn GenK getConstK goodFn2
+                                   bdm dmn preDm sufDm ls noDup eq_refl bdr rn preR
+                                   sufR eq_refl noDupMeth noDupRule);
+                       pose proof (@inlineGenGenDmToRule_ModEquiv_NoFilt
+                                     m mEquiv A strA goodFn GenK getConstK goodFn2
+                                     bdm dmn preDm sufDm ls noDup eq_refl bdr rn preR
+                                     sufR eq_refl noDupMeth noDupRule);
+                       clear noDupMeth noDupRule
+                 end
+             end
   end.
 
-Ltac inlineGenDmGenRule_NoFilt m mEquiv dm r :=
-  let noDupMeth := fresh in
-  let noDupRule := fresh in
-  assert (noDupMeth: NoDup (map getMetaMethName (metaMeths m))) by
-    (subst; simpl; clear; noDup_tac);
-    assert (noDupRule: NoDup (map getMetaRuleName (metaRules m))) by
-      (subst; simpl; clear; noDup_tac);
-    let dmTriple := eval simpl in (findDm dm nil (metaMeths m)) in
-        let rTriple := eval simpl in (findR r nil (metaRules m)) in
-            match dmTriple with
-              | Some (?preDm, @RepMeth ?A ?strA ?goodFn ?GenK ?getConstK
-                                       ?goodFn2 ?bdm ?dmn ?ls ?noDup, ?sufDm) =>
-                match rTriple with
-                  | Some (?preR, @RepRule ?A ?strA ?goodFn ?GenK ?getConstK
-                                          ?goodFn2 ?bdr ?rn ?ls ?noDup, ?sufR) =>
-                    let m'Ref := fresh in
-                    let m'Equiv := fresh in
-                    pose proof (@inlineGenGenDmToRule_traceRefines_NoFilt
-                                  m A strA goodFn GenK getConstK goodFn2
-                                  bdm dmn preDm sufDm ls noDup eq_refl bdr rn preR
-                                  sufR eq_refl noDupMeth noDupRule);
-                      pose proof (@inlineGenGenDmToRule_ModEquiv_NoFilt
-                                    m mEquiv A strA goodFn GenK getConstK goodFn2
-                                    bdm dmn preDm sufDm ls noDup eq_refl bdr rn preR
-                                    sufR eq_refl noDupMeth noDupRule);
-                      clear noDupMeth noDupRule
-                end
-            end.
+Ltac inlineGenDmGenRule_Filt dm r :=
+  match goal with
+    | m := {| metaRegs := _; metaRules := ?rls; metaMeths := ?mts |},        
+           mEquiv: forall ty, MetaModEquiv ty typeUT ?m |- _ =>
+           let noDupMeth := fresh in
+           let noDupRule := fresh in
+           assert (noDupMeth: NoDup (map getMetaMethName mts)) by
+               ( (subst; simpl; clear; noDup_tac));
+             assert (noDupRule: NoDup (map getMetaRuleName rls)) by
+               ( (subst; simpl; clear; noDup_tac));
+             let dmTriple := find dm (@nil MetaMeth) mts in
+             let rTriple := find r (@nil MetaRule) rls in
+             match dmTriple with
+               | (?preDm, @RepMeth ?A ?strA ?goodFn ?GenK ?getConstK
+                                   ?goodFn2 ?bdm ?dmn ?ls ?noDup, ?sufDm) =>
+                 match rTriple with
+                   | (?preR, @RepRule ?A ?strA ?goodFn ?GenK ?getConstK
+                                      ?goodFn2 ?bdr ?rn ?ls ?noDup, ?sufR) =>
+                     let H3 := fresh in
+                     let H4 := fresh in
+                     let H5 := fresh in
+                     assert
+                       (H3:
+                          forall r',
+                            In r' (preR ++ sufR) ->
+                            match r' with
+                              | OneRule _ _ => true
+                              | RepRule _ _ _ _ _ _ bgenB _ _ _ =>
+                                noCallDmSigGenA (bgenB typeUT)
+                                                {| isRep := true; nameRec := dmn |}
+                                                (projT1 bdm)
+                            end = true) by
+                         ( (intro;
+                                    apply boolListReflection with
+                                    (f := (fun r' =>
+                                             match r' with
+                                               | OneRule _ _ => true
+                                               | RepRule _ _ _ _ _ _ bgenB _ _ _ =>
+                                                 noCallDmSigGenA (bgenB typeUT)
+                                                                 {| isRep := true; nameRec := dmn |}
+                                                                 (projT1 bdm)
+                                             end)); apply eq_refl));
+                       assert
+                         (H4:
+                            forall dm',
+                              In dm' (metaMeths m) ->
+                              match dm' with
+                                | OneMeth _ _ => true
+                                | RepMeth _ _ _ _ _ _ bgenB _ _ _ =>
+                                  noCallDmSigGenA (projT2 bgenB typeUT tt)
+                                                  {| isRep := true; nameRec := dmn |}
+                                                  (projT1 bdm)
+                              end = true) by
+                         ( (intro;
+                                    apply boolListReflection with
+                                    (f := (fun dm' =>
+                                             match dm' with
+                                               | OneMeth _ _ => true
+                                               | RepMeth _ _ _ _ _ _ bgenB _ _ _ =>
+                                                 noCallDmSigGenA (projT2 bgenB typeUT tt)
+                                                                 {| isRep := true; nameRec := dmn |}
+                                                                 (projT1 bdm)
+                                             end)); apply eq_refl));
+                       assert
+                         (H5: exists call : NameRecIdx,
+                                In call (getCallsGenA (bdr typeUT)) /\
+                                nameVal (nameRec call) = nameVal dmn /\ isRep call = true) by
+                           ( (eexists {| isRep := true;
+                                                 nameRec := {| nameVal := nameVal dmn;
+                                                               goodName := _ |} |};
+                                      split; [
+                                        simpl; tauto | split; reflexivity]));
+                       pose proof (@inlineGenGenDmToRule_traceRefines_Filt'
+                                     m mEquiv A strA goodFn GenK getConstK goodFn2
+                                     bdm dmn preDm sufDm ls noDup eq_refl bdr rn preR
+                                     sufR eq_refl noDupMeth noDupRule H3 H4 H5);
+                       pose proof (@inlineGenGenDmToRule_ModEquiv_Filt'
+                                     m mEquiv A strA goodFn GenK getConstK goodFn2
+                                     bdm dmn preDm sufDm ls noDup eq_refl bdr rn preR
+                                     sufR eq_refl noDupMeth noDupRule H4);
+                       clear noDupMeth noDupRule H3 H4 H5
+                 end
+             end
+  end.
 
-Ltac inlineGenDmGenRule_Filt m mEquiv dm r :=
-  let noDupMeth := fresh in
-  let noDupRule := fresh in
-  assert (noDupMeth: NoDup (map getMetaMethName (metaMeths m))) by
-      (subst; simpl; clear; noDup_tac);
-    assert (noDupRule: NoDup (map getMetaRuleName (metaRules m))) by
-      (subst; simpl; clear; noDup_tac);
-    let dmTriple := eval simpl in (findDm dm nil (metaMeths m)) in
-        let rTriple := eval simpl in (findR r nil (metaRules m)) in
-            match dmTriple with
-              | Some (?preDm, @RepMeth ?A ?strA ?goodFn ?GenK ?getConstK
-                                       ?goodFn2 ?bdm ?dmn ?ls ?noDup, ?sufDm) =>
-                match rTriple with
-                  | Some (?preR, @RepRule ?A ?strA ?goodFn ?GenK ?getConstK
-                                          ?goodFn2 ?bdr ?rn ?ls ?noDup, ?sufR) =>
-                    let H3 := fresh in
-                    let H4 := fresh in
-                    let H5 := fresh in
-                    assert
-                      (H3:
-                         forall r',
-                           In r' (preR ++ sufR) ->
-                           match r' with
-                             | OneRule _ _ => true
-                             | RepRule _ _ _ _ _ _ bgenB _ _ _ =>
-                               noCallDmSigGenA (bgenB typeUT)
-                                               {| isRep := true; nameRec := dmn |}
-                                               (projT1 bdm)
-                           end = true) by
-                        (intro;
-                         apply boolListReflection with
-                         (f := (fun r' =>
-                                  match r' with
-                                    | OneRule _ _ => true
-                                    | RepRule _ _ _ _ _ _ bgenB _ _ _ =>
-                                      noCallDmSigGenA (bgenB typeUT)
-                                                      {| isRep := true; nameRec := dmn |}
-                                                      (projT1 bdm)
-                                  end)); apply eq_refl);
-                      assert
-                        (H4:
-                           forall dm',
-                             In dm' (metaMeths m) ->
-                             match dm' with
-                               | OneMeth _ _ => true
-                               | RepMeth _ _ _ _ _ _ bgenB _ _ _ =>
-                                 noCallDmSigGenA (projT2 bgenB typeUT tt)
-                                                 {| isRep := true; nameRec := dmn |}
-                                                 (projT1 bdm)
-                             end = true) by
-                        (intro;
-                         apply boolListReflection with
-                         (f := (fun dm' =>
-                                  match dm' with
-                                    | OneMeth _ _ => true
-                                    | RepMeth _ _ _ _ _ _ bgenB _ _ _ =>
-                                      noCallDmSigGenA (projT2 bgenB typeUT tt)
-                                                      {| isRep := true; nameRec := dmn |}
-                                                      (projT1 bdm)
-                                  end)); apply eq_refl);
-                      assert
-                        (H5: exists call : NameRecIdx,
-                               In call (getCallsGenA (bdr typeUT)) /\
-                               nameVal (nameRec call) = nameVal dmn /\ isRep call = true) by
-                          (eexists {| isRep := true;
-                                      nameRec := {| nameVal := nameVal dmn;
-                                                    goodName := _ |} |};
-                           split; [
-                             simpl; tauto | split; reflexivity]);
-                      pose proof (@inlineGenGenDmToRule_traceRefines_Filt'
-                                    m mEquiv A strA goodFn GenK getConstK goodFn2
-                                    bdm dmn preDm sufDm ls noDup eq_refl bdr rn preR
-                                    sufR eq_refl noDupMeth noDupRule H3 H4 H5);
-                        pose proof (@inlineGenGenDmToRule_ModEquiv_Filt'
-                                      m mEquiv A strA goodFn GenK getConstK goodFn2
-                                      bdm dmn preDm sufDm ls noDup eq_refl bdr rn preR
-                                      sufR eq_refl noDupMeth noDupRule H4);
-                        clear noDupMeth noDupRule H3 H4 H5
-                end
-            end.
-
-Ltac inlineSinDmGenRule_NoFilt m mEquiv dm r :=
-  let noDupMeth := fresh in
-  let noDupRule := fresh in
-  assert (noDupMeth: NoDup (map getMetaMethName (metaMeths m))) by
-      (subst; simpl; clear; noDup_tac);
-    assert (noDupRule: NoDup (map getMetaRuleName (metaRules m))) by
-      (subst; simpl; clear; noDup_tac);
-    let dmTriple := eval simpl in (findDm dm nil (metaMeths m)) in
-        let rTriple := eval simpl in (findR r nil (metaRules m)) in
-            match dmTriple with
-              | Some (?preDm, @OneMeth ?bdm ?dmn, ?sufDm) =>
-                match rTriple with
-                  | Some (?preR, @RepRule ?A ?strA ?goodFn ?GenK ?getConstK
-                                          ?goodFn2 ?bdr ?rn ?ls ?noDup, ?sufR) =>
-                    let m'Ref := fresh in
-                    let m'Equiv := fresh in
-                    pose proof (@inlineGenSinDmToRule_traceRefines_NoFilt
-                                  m A strA goodFn GenK getConstK goodFn2
-                                  bdm dmn preDm sufDm ls noDup eq_refl bdr rn preR
-                                  sufR eq_refl noDupMeth noDupRule);
-                      pose proof (@inlineGenSinDmToRule_ModEquiv_NoFilt
-                                    m mEquiv A strA goodFn GenK getConstK goodFn2
-                                    bdm dmn preDm sufDm ls noDup eq_refl bdr rn preR
-                                    sufR eq_refl noDupMeth noDupRule);
-                      clear noDupMeth noDupRule
-                end
-            end.
+Ltac inlineSinDmGenRule_NoFilt dm r :=
+  match goal with
+    | m := {| metaRegs := _; metaRules := ?rls; metaMeths := ?mts |},        
+           mEquiv: forall ty, MetaModEquiv ty typeUT ?m |- _ =>
+           let noDupMeth := fresh in
+           let noDupRule := fresh in
+           assert (noDupMeth: NoDup (map getMetaMethName mts)) by
+               ( (subst; simpl; clear; noDup_tac));
+             assert (noDupRule: NoDup (map getMetaRuleName rls)) by
+               ( (subst; simpl; clear; noDup_tac));
+             let dmTriple := find dm (@nil MetaMeth) mts in
+             let rTriple := find r (@nil MetaRule) rls in
+             match dmTriple with
+               | (?preDm, @OneMeth ?bdm ?dmn, ?sufDm) =>
+                 match rTriple with
+                   | (?preR, @RepRule ?A ?strA ?goodFn ?GenK ?getConstK
+                                      ?goodFn2 ?bdr ?rn ?ls ?noDup, ?sufR) =>
+                     pose proof (@inlineGenSinDmToRule_traceRefines_NoFilt
+                                   m A strA goodFn GenK getConstK goodFn2
+                                   bdm dmn preDm sufDm ls noDup eq_refl bdr rn preR
+                                   sufR eq_refl noDupMeth noDupRule);
+                       pose proof (@inlineGenSinDmToRule_ModEquiv_NoFilt
+                                     m mEquiv A strA goodFn GenK getConstK goodFn2
+                                     bdm dmn preDm sufDm ls noDup eq_refl bdr rn preR
+                                     sufR eq_refl noDupMeth noDupRule);
+                       clear noDupMeth noDupRule
+                 end
+             end
+  end.
 
 Theorem notNilNatList: forall n,
                          getNatListToN (Word.wordToNat (Word.wones n)) <> nil.
@@ -199,199 +175,217 @@ Proof.
   induction n; simpl in *; unfold not; intros; discriminate.
 Qed.
 
-Ltac inlineSinDmGenRule_Filt m mEquiv dm r :=
-  let noDupMeth := fresh in
-  let noDupRule := fresh in
-  assert (noDupMeth: NoDup (map getMetaMethName (metaMeths m))) by
-      (subst; simpl; clear; noDup_tac);
-    assert (noDupRule: NoDup (map getMetaRuleName (metaRules m))) by
-      (subst; simpl; clear; noDup_tac);
-    let dmTriple := eval simpl in (findDm dm nil (metaMeths m)) in
-        let rTriple := eval simpl in (findR r nil (metaRules m)) in
-            match dmTriple with
-              | Some (?preDm, @OneMeth ?bdm ?dmn, ?sufDm) =>
-                match rTriple with
-                  | Some (?preR, @RepRule ?A ?strA ?goodFn ?GenK ?getConstK
-                                          ?goodFn2 ?bdr ?rn ?ls ?noDup, ?sufR) =>
-                    let H3 := fresh in
-                    let H4 := fresh in
-                    let H5 := fresh in
-                    let H6 := fresh in
-                    assert
-                      (H3:
-                         forall r',
-                           In r' (preR ++ sufR) ->
-                           match r' with
-                             | OneRule bgenB _ =>
-                               noCallDmSigSinA (bgenB typeUT) dmn (projT1 bdm)
-                             | RepRule _ _ _ _ _ _ bgenB _ _ _ =>
-                               noCallDmSigGenA (bgenB typeUT)
-                                               {| isRep := false; nameRec := dmn |}
-                                               (projT1 bdm)
-                           end = true) by
-                        (intro;
-                         apply boolListReflection with
-                         (f := (fun r' =>
-                                  match r' with
-                                    | OneRule bgenB _ =>
-                                      noCallDmSigSinA (bgenB typeUT) dmn (projT1 bdm)
-                                    | RepRule _ _ _ _ _ _ bgenB _ _ _ =>
-                                      noCallDmSigGenA (bgenB typeUT)
-                                                      {| isRep := false; nameRec := dmn |}
-                                                      (projT1 bdm)
-                                  end)); apply eq_refl);
-                      assert
-                        (H4:
-                           forall dm',
-                             In dm' (metaMeths m) ->
-                             match dm' with
-                               | OneMeth bgenB _ =>
-                                 noCallDmSigSinA (projT2 bgenB typeUT tt) dmn (projT1 bdm)
-                               | RepMeth _ _ _ _ _ _ bgenB _ _ _ =>
-                                 noCallDmSigGenA (projT2 bgenB typeUT tt)
-                                                 {| isRep := false; nameRec := dmn |}
-                                                 (projT1 bdm)
-                             end = true) by
-                        (intro;
-                         apply boolListReflection with
-                         (f := (fun dm' =>
-                                  match dm' with
-                                    | OneMeth bgenB _ =>
-                                      noCallDmSigSinA (projT2 bgenB typeUT tt) dmn (projT1 bdm)
-                                    | RepMeth _ _ _ _ _ _ bgenB _ _ _ =>
-                                      noCallDmSigGenA (projT2 bgenB typeUT tt)
-                                                      {| isRep := false; nameRec := dmn |}
-                                                      (projT1 bdm)
-                                  end)); apply eq_refl);
-                      assert
-                        (H5: exists call : NameRecIdx,
-                               In call (getCallsGenA (bdr typeUT)) /\
-                               nameVal (nameRec call) = nameVal dmn /\ isRep call = false) by
-                          (eexists {| isRep := false;
-                                      nameRec := {| nameVal := nameVal dmn;
-                                                    goodName := _ |} |};
-                           split; [
-                             simpl; tauto | split; reflexivity]);
-                      assert
-                        (H6: ls <> nil) by (apply notNilNatList; auto);
-                      pose proof (@inlineGenSinDmToRule_traceRefines_Filt'
-                                    m mEquiv A strA goodFn GenK getConstK goodFn2
-                                    bdm dmn preDm sufDm ls H6 noDup eq_refl bdr rn preR
-                                    sufR eq_refl noDupMeth noDupRule H3 H4 H5);
-                        pose proof (@inlineGenSinDmToRule_ModEquiv_Filt'
-                                      m mEquiv A strA goodFn GenK getConstK goodFn2
-                                      bdm dmn preDm sufDm ls noDup eq_refl bdr rn preR
-                                      sufR eq_refl noDupMeth noDupRule H4);
-                        clear noDupMeth noDupRule H3 H4 H5 H6
-                end
-            end.
+Ltac inlineSinDmGenRule_Filt dm r :=
+  match goal with
+    | m := {| metaRegs := _; metaRules := ?rls; metaMeths := ?mts |},        
+           mEquiv: forall ty, MetaModEquiv ty typeUT ?m |- _ =>
+           let noDupMeth := fresh in
+           let noDupRule := fresh in
+           assert (noDupMeth: NoDup (map getMetaMethName mts)) by
+               ( (subst; simpl; clear; noDup_tac));
+             assert (noDupRule: NoDup (map getMetaRuleName rls)) by
+               ( (subst; simpl; clear; noDup_tac));
+             let dmTriple := find dm (@nil MetaMeth) mts in
+             let rTriple := find r (@nil MetaRule) rls in
+             match dmTriple with
+               | (?preDm, @OneMeth ?bdm ?dmn, ?sufDm) =>
+                 match rTriple with
+                   | (?preR, @RepRule ?A ?strA ?goodFn ?GenK ?getConstK
+                                      ?goodFn2 ?bdr ?rn ?ls ?noDup, ?sufR) =>
+                     let H3 := fresh in
+                     let H4 := fresh in
+                     let H5 := fresh in
+                     let H6 := fresh in
+                     assert
+                       (H3:
+                          forall r',
+                            In r' (preR ++ sufR) ->
+                            match r' with
+                              | OneRule bgenB _ =>
+                                noCallDmSigSinA (bgenB typeUT) dmn (projT1 bdm)
+                              | RepRule _ _ _ _ _ _ bgenB _ _ _ =>
+                                noCallDmSigGenA (bgenB typeUT)
+                                                {| isRep := false; nameRec := dmn |}
+                                                (projT1 bdm)
+                            end = true) by
+                         ( (intro;
+                                    apply boolListReflection with
+                                    (f := (fun r' =>
+                                             match r' with
+                                               | OneRule bgenB _ =>
+                                                 noCallDmSigSinA (bgenB typeUT) dmn (projT1 bdm)
+                                               | RepRule _ _ _ _ _ _ bgenB _ _ _ =>
+                                                 noCallDmSigGenA (bgenB typeUT)
+                                                                 {| isRep := false;
+                                                                    nameRec := dmn |}
+                                                                 (projT1 bdm)
+                                             end)); apply eq_refl));
+                       assert
+                         (H4:
+                            forall dm',
+                              In dm' (metaMeths m) ->
+                              match dm' with
+                                | OneMeth bgenB _ =>
+                                  noCallDmSigSinA (projT2 bgenB typeUT tt) dmn (projT1 bdm)
+                                | RepMeth _ _ _ _ _ _ bgenB _ _ _ =>
+                                  noCallDmSigGenA (projT2 bgenB typeUT tt)
+                                                  {| isRep := false; nameRec := dmn |}
+                                                  (projT1 bdm)
+                              end = true) by
+                         ( (intro;
+                                    apply boolListReflection with
+                                    (f := (fun dm' =>
+                                             match dm' with
+                                               | OneMeth bgenB _ =>
+                                                 noCallDmSigSinA (projT2 bgenB typeUT tt)
+                                                                 dmn (projT1 bdm)
+                                               | RepMeth _ _ _ _ _ _ bgenB _ _ _ =>
+                                                 noCallDmSigGenA (projT2 bgenB typeUT tt)
+                                                                 {| isRep := false;
+                                                                    nameRec := dmn |}
+                                                                 (projT1 bdm)
+                                             end)); apply eq_refl));
+                       assert
+                         (H5: exists call : NameRecIdx,
+                                In call (getCallsGenA (bdr typeUT)) /\
+                                nameVal (nameRec call) = nameVal dmn /\ isRep call = false) by
+                           ( (eexists {| isRep := false;
+                                                 nameRec := {| nameVal := nameVal dmn;
+                                                               goodName := _ |} |};
+                                      split; [
+                                        simpl; tauto | split; reflexivity]));
+                       assert
+                         (H6: ls <> nil) by ( (apply notNilNatList; auto));
+                       pose proof (@inlineGenSinDmToRule_traceRefines_Filt'
+                                     m mEquiv A strA goodFn GenK getConstK goodFn2
+                                     bdm dmn preDm sufDm ls H6 noDup eq_refl bdr rn preR
+                                     sufR eq_refl noDupMeth noDupRule H3 H4 H5);
+                       pose proof (@inlineGenSinDmToRule_ModEquiv_Filt'
+                                     m mEquiv A strA goodFn GenK getConstK goodFn2
+                                     bdm dmn preDm sufDm ls noDup eq_refl bdr rn preR
+                                     sufR eq_refl noDupMeth noDupRule H4);
+                       clear noDupMeth noDupRule H3 H4 H5 H6
+                 end
+             end
+  end.
 
-Ltac inlineSinDmSinRule_NoFilt m mEquiv dm r :=
-  let noDupMeth := fresh in
-  let noDupRule := fresh in
-  assert (noDupMeth: NoDup (map getMetaMethName (metaMeths m))) by
-      (subst; simpl; clear; noDup_tac);
-    assert (noDupRule: NoDup (map getMetaRuleName (metaRules m))) by
-      (subst; simpl; clear; noDup_tac);
-    let dmTriple := eval simpl in (findDm dm nil (metaMeths m)) in
-        let rTriple := eval simpl in (findR r nil (metaRules m)) in
-            match dmTriple with
-              | Some (?preDm, @OneMeth ?bdm ?dmn, ?sufDm) =>
-                match rTriple with
-                  | Some (?preR, @OneRule ?bdr ?rn, ?sufR) =>
-                    let m'Ref := fresh in
-                    let m'Equiv := fresh in
-                    pose proof (@inlineSinSinDmToRule_traceRefines_NoFilt
-                                  m
-                                  bdm dmn preDm sufDm eq_refl bdr rn preR
-                                  sufR eq_refl noDupMeth noDupRule);
-                      pose proof (@inlineSinSinDmToRule_ModEquiv_NoFilt
-                                    m mEquiv
-                                    bdm dmn preDm sufDm eq_refl bdr rn preR
-                                    sufR eq_refl noDupMeth noDupRule);
-                      clear noDupMeth noDupRule
-                end
-            end.
+Ltac inlineSinDmSinRule_NoFilt dm r :=
+  match goal with
+    | m := {| metaRegs := _; metaRules := ?rls; metaMeths := ?mts |},        
+           mEquiv: forall ty, MetaModEquiv ty typeUT ?m |- _ =>
+           let noDupMeth := fresh in
+           let noDupRule := fresh in
+           assert (noDupMeth: NoDup (map getMetaMethName mts)) by
+               ( (subst; simpl; clear; noDup_tac));
+             assert (noDupRule: NoDup (map getMetaRuleName rls)) by
+               ( (subst; simpl; clear; noDup_tac));
+             let dmTriple := find dm (@nil MetaMeth) mts in
+             let rTriple := find r (@nil MetaRule) rls in
+             match dmTriple with
+               | (?preDm, @OneMeth ?bdm ?dmn, ?sufDm) =>
+                 match rTriple with
+                   | (?preR, @OneRule ?bdr ?rn, ?sufR) =>
+                     pose proof (@inlineSinSinDmToRule_traceRefines_NoFilt
+                                   m
+                                   bdm dmn preDm sufDm eq_refl bdr rn preR
+                                   sufR eq_refl noDupMeth noDupRule);
+                       pose proof (@inlineSinSinDmToRule_ModEquiv_NoFilt
+                                     m mEquiv
+                                     bdm dmn preDm sufDm eq_refl bdr rn preR
+                                     sufR eq_refl noDupMeth noDupRule);
+                       clear noDupMeth noDupRule
+                 end
+             end
+  end.
+
+Ltac inlineSinDmSinRule_Filt dm r :=
+  match goal with
+    | m := {| metaRegs := _; metaRules := ?rls; metaMeths := ?mts |},        
+           mEquiv: forall ty, MetaModEquiv ty typeUT ?m |- _ =>
+           let noDupMeth := fresh in
+           let noDupRule := fresh in
+           assert (noDupMeth: NoDup (map getMetaMethName mts)) by
+               ( (subst; simpl; clear; noDup_tac));
+             assert (noDupRule: NoDup (map getMetaRuleName rls)) by
+               ( (subst; simpl; clear; noDup_tac));
+             let dmTriple := find dm (@nil MetaMeth) mts in
+             let rTriple := find r (@nil MetaRule) rls in
+             match dmTriple with
+               | (?preDm, @OneMeth ?bdm ?dmn, ?sufDm) =>
+                 match rTriple with
+                   | (?preR, @OneRule ?bdr ?rn, ?sufR) =>
+                     let H3 := fresh in
+                     let H4 := fresh in
+                     let H5 := fresh in
+                     assert
+                       (H3:
+                          forall r',
+                            In r' (preR ++ sufR) ->
+                            match r' with
+                              | OneRule bgenB _ =>
+                                noCallDmSigSinA (bgenB typeUT) dmn (projT1 bdm)
+                              | RepRule _ _ _ _ _ _ bgenB _ _ _ =>
+                                noCallDmSigGenA (bgenB typeUT)
+                                                {| isRep := false; nameRec := dmn |}
+                                                (projT1 bdm)
+                            end = true) by
+                         ( (intro;
+                                    apply boolListReflection with
+                                    (f := (fun r' =>
+                                             match r' with
+                                               | OneRule bgenB _ =>
+                                                 noCallDmSigSinA (bgenB typeUT) dmn (projT1 bdm)
+                                               | RepRule _ _ _ _ _ _ bgenB _ _ _ =>
+                                                 noCallDmSigGenA (bgenB typeUT)
+                                                                 {| isRep := false;
+                                                                    nameRec := dmn |}
+                                                                 (projT1 bdm)
+                                             end)); apply eq_refl));
+                       assert
+                         (H4:
+                            forall dm',
+                              In dm' (metaMeths m) ->
+                              match dm' with
+                                | OneMeth bgenB _ =>
+                                  noCallDmSigSinA (projT2 bgenB typeUT tt) dmn (projT1 bdm)
+                                | RepMeth _ _ _ _ _ _ bgenB _ _ _ =>
+                                  noCallDmSigGenA (projT2 bgenB typeUT tt)
+                                                  {| isRep := false; nameRec := dmn |}
+                                                  (projT1 bdm)
+                              end = true) by
+                         ( (intro;
+                                    apply boolListReflection with
+                                    (f := (fun dm' =>
+                                             match dm' with
+                                               | OneMeth bgenB _ =>
+                                                 noCallDmSigSinA (projT2 bgenB typeUT tt)
+                                                                 dmn (projT1 bdm)
+                                               | RepMeth _ _ _ _ _ _ bgenB _ _ _ =>
+                                                 noCallDmSigGenA (projT2 bgenB typeUT tt)
+                                                                 {| isRep := false;
+                                                                    nameRec := dmn |}
+                                                                 (projT1 bdm)
+                                             end)); apply eq_refl));
+                       assert
+                         (H5: exists call : NameRec,
+                                In call (getCallsSinA (bdr typeUT)) /\
+                                nameVal call = nameVal dmn) by
+                           ( (eexists {| nameVal := nameVal dmn;
+                                                 goodName := _ |};
+                                      split; [
+                                        simpl; tauto | reflexivity]));
+                       pose proof (@inlineSinSinDmToRule_traceRefines_Filt'
+                                     m mEquiv
+                                     bdm dmn preDm sufDm eq_refl bdr rn preR
+                                     sufR eq_refl noDupMeth noDupRule H3 H4 H5);
+                       pose proof (@inlineSinSinDmToRule_ModEquiv_Filt'
+                                     m mEquiv
+                                     bdm dmn preDm sufDm eq_refl bdr rn preR
+                                     sufR eq_refl noDupMeth noDupRule H4);
+                       clear noDupMeth noDupRule H3 H4 H5
+                 end
+             end
+  end.
 
 
-Ltac inlineSinDmSinRule_Filt m mEquiv dm r :=
-  let noDupMeth := fresh in
-  let noDupRule := fresh in
-  assert (noDupMeth: NoDup (map getMetaMethName (metaMeths m))) by
-      (subst; simpl; clear; noDup_tac);
-    assert (noDupRule: NoDup (map getMetaRuleName (metaRules m))) by
-      (subst; simpl; clear; noDup_tac);
-    let dmTriple := eval simpl in (findDm dm nil (metaMeths m)) in
-        let rTriple := eval simpl in (findR r nil (metaRules m)) in
-            match dmTriple with
-              | Some (?preDm, @OneMeth ?bdm ?dmn, ?sufDm) =>
-                match rTriple with
-                  | Some (?preR, @OneRule ?bdr ?rn, ?sufR) =>
-                    let H3 := fresh in
-                    let H4 := fresh in
-                    let H5 := fresh in
-                    assert
-                      (H3:
-                         forall r',
-                           In r' (preR ++ sufR) ->
-                           match r' with
-                             | OneRule bgenB _ =>
-                               noCallDmSigSinA (bgenB typeUT) dmn (projT1 bdm)
-                             | RepRule _ _ _ _ _ _ bgenB _ _ _ =>
-                               noCallDmSigGenA (bgenB typeUT)
-                                               {| isRep := false; nameRec := dmn |}
-                                               (projT1 bdm)
-                           end = true) by
-                        (intro;
-                         apply boolListReflection with
-                         (f := (fun r' =>
-                                  match r' with
-                                    | OneRule bgenB _ =>
-                                      noCallDmSigSinA (bgenB typeUT) dmn (projT1 bdm)
-                                    | RepRule _ _ _ _ _ _ bgenB _ _ _ =>
-                                      noCallDmSigGenA (bgenB typeUT)
-                                                      {| isRep := false; nameRec := dmn |}
-                                                      (projT1 bdm)
-                                  end)); apply eq_refl);
-                      assert
-                        (H4:
-                           forall dm',
-                             In dm' (metaMeths m) ->
-                             match dm' with
-                               | OneMeth bgenB _ =>
-                                 noCallDmSigSinA (projT2 bgenB typeUT tt) dmn (projT1 bdm)
-                               | RepMeth _ _ _ _ _ _ bgenB _ _ _ =>
-                                 noCallDmSigGenA (projT2 bgenB typeUT tt)
-                                                 {| isRep := false; nameRec := dmn |}
-                                                 (projT1 bdm)
-                             end = true) by
-                        (intro;
-                         apply boolListReflection with
-                         (f := (fun dm' =>
-                                  match dm' with
-                                    | OneMeth bgenB _ =>
-                                      noCallDmSigSinA (projT2 bgenB typeUT tt) dmn (projT1 bdm)
-                                    | RepMeth _ _ _ _ _ _ bgenB _ _ _ =>
-                                      noCallDmSigGenA (projT2 bgenB typeUT tt)
-                                                      {| isRep := false; nameRec := dmn |}
-                                                      (projT1 bdm)
-                                  end)); apply eq_refl);
-                      assert
-                        (H5: exists call : NameRec,
-                               In call (getCallsSinA (bdr typeUT)) /\
-                               nameVal call = nameVal dmn) by
-                          (eexists {| nameVal := nameVal dmn;
-                                      goodName := _ |};
-                           split; [
-                             simpl; tauto | reflexivity]);
-                      pose proof (@inlineSinSinDmToRule_traceRefines_Filt'
-                                    m mEquiv
-                                    bdm dmn preDm sufDm eq_refl bdr rn preR
-                                    sufR eq_refl noDupMeth noDupRule H3 H4 H5);
-                        pose proof (@inlineSinSinDmToRule_ModEquiv_Filt'
-                                      m mEquiv
-                                      bdm dmn preDm sufDm eq_refl bdr rn preR
-                                      sufR eq_refl noDupMeth noDupRule H4);
-                        clear noDupMeth noDupRule H3 H4 H5
-                end
-            end.
+Close Scope string.
